Tidied up examples

Coq/VeracityLogicV3.v
@@ -536,6 +536,8 @@ Definition Q := Actor "Q".
 Definition C1 := AtomicClaim "C_1".
 Definition C2 := AtomicClaim "C_2".
 Definition C3 := AtomicClaim "C_3".
+Definition C4 := AtomicClaim "C_4".
+Definition C5 := AtomicClaim "C_5".
 
 Definition concreteProofTreeExampleWith2Conjuncts : 
 proofTreeOf [l \by P \in C1; s \by P \in C2]
@@ -884,22 +886,22 @@ solve [ eapply leaf | eapply assume | eapply assume_bot | eapply bot_elim | eapp
     simpl; Control.plus (
      fun () => Control.plus (fun () => fail)
      
-     (fun _ => Control.plus (fun () => try (( eapply leaf); proofSearch (Int.sub max_depth 1)); (maybePrintMessage "Trying leaf"); proofSearch (Int.sub max_depth 1))
-     (fun _ => Control.plus (fun () => try (( eapply assume); proofSearch (Int.sub max_depth 1)); (maybePrintMessage "Trying assume"); proofSearch (Int.sub max_depth 1))
-     (fun _ => Control.plus (fun () => try (( eapply and_intro; simpl in *); proofSearch (Int.sub max_depth 1)); (maybePrintMessage "Trying and_intro"); proofSearch (Int.sub max_depth 1))
-     (fun _ => Control.plus (fun () => try (( eapply or_intro1); proofSearch (Int.sub max_depth 1)); (maybePrintMessage "Trying or_intro1"); proofSearch (Int.sub max_depth 1))
-     (fun _ => Control.plus (fun () => try (( eapply or_intro2); proofSearch (Int.sub max_depth 1)); (maybePrintMessage "Trying or_intro2"); proofSearch (Int.sub max_depth 1))
-     (* (fun _ => Control.plus (fun () => try (( eapply and_elim1); proofSearch (Int.sub max_depth 1)); (maybePrintMessage "Trying and_elim1"); proofSearch (Int.sub max_depth 1)) *)
-     (* (fun _ => Control.plus (fun () => try (( eapply and_elim2); proofSearch (Int.sub max_depth 1)); (maybePrintMessage "Trying and_elim2"); proofSearch (Int.sub max_depth 1)) *)
-     (* (fun _ => Control.plus (fun () => try (( eapply or_elim1); proofSearch (Int.sub max_depth 1)); (maybePrintMessage "Trying or_elim1"); proofSearch (Int.sub max_depth 1)) *)
-     (* (fun _ => Control.plus (fun () => try (( eapply or_elim2); proofSearch (Int.sub max_depth 1)); (maybePrintMessage "Trying or_elim2"); proofSearch (Int.sub max_depth 1)) *)
-     (fun _ => Control.plus (fun () => try (( eapply trust); proofSearch (Int.sub max_depth 1)); (maybePrintMessage "Trying trust"); proofSearch (Int.sub max_depth 1))
-     (fun _ => Control.plus (fun () => try (( eapply impl_intro); proofSearch (Int.sub max_depth 1)); (maybePrintMessage "Trying impl_intro"); proofSearch (Int.sub max_depth 1))
-     (* (fun _ => Control.plus (fun () => try (( eapply bot_elim); proofSearch (Int.sub max_depth 1)); (maybePrintMessage "Trying bot_elim"); proofSearch (Int.sub max_depth 1)) *)
-     (* (fun _ => Control.plus (fun () => try (( eapply assume_bot); proofSearch (Int.sub max_depth 1)); (maybePrintMessage "Trying assume_bot"); proofSearch (Int.sub max_depth 1)) *)
-     (* (fun _ => Control.plus (fun () => try (( eapply admit ); proofSearch (Int.sub max_depth 1)); (maybePrintMessage "Trying admit"); proofSearch (Int.sub max_depth 1)) *)
+     (fun _ => Control.plus (fun () => ( try (eapply trust); proofSearch (Int.sub max_depth 1)); (maybePrintMessage "Trying trust"); proofSearch (Int.sub max_depth 1))
+     (fun _ => Control.plus (fun () => ( try (eapply leaf); proofSearch (Int.sub max_depth 1)); (maybePrintMessage "Trying leaf"); proofSearch (Int.sub max_depth 1))
+     (fun _ => Control.plus (fun () => ( try (eapply assume ); proofSearch (Int.sub max_depth 1)); (maybePrintMessage "Trying assume"); proofSearch (Int.sub max_depth 1))
+     (fun _ => Control.plus (fun () => ( try (eapply and_intro); proofSearch (Int.sub max_depth 1)); (maybePrintMessage "Trying and_intro"); proofSearch (Int.sub max_depth 1))
+     (* (fun _ => Control.plus (fun () => ( try (eapply or_intro1); proofSearch (Int.sub max_depth 1)); (maybePrintMessage "Trying or_intro1"); proofSearch (Int.sub max_depth 1)) *)
+     (* (fun _ => Control.plus (fun () => ( try (eapply or_intro2); proofSearch (Int.sub max_depth 1)); (maybePrintMessage "Trying or_intro2"); proofSearch (Int.sub max_depth 1)) *)
+     (* (fun _ => Control.plus (fun () => ( try (eapply and_elim1); proofSearch (Int.sub max_depth 1)); (maybePrintMessage "Trying and_elim1"); proofSearch (Int.sub max_depth 1)) *)
+     (* (fun _ => Control.plus (fun () => ( try (eapply and_elim2); proofSearch (Int.sub max_depth 1)); (maybePrintMessage "Trying and_elim2"); proofSearch (Int.sub max_depth 1)) *)
+     (* (fun _ => Control.plus (fun () => ( try (eapply or_elim1); proofSearch (Int.sub max_depth 1)); (maybePrintMessage "Trying or_elim1"); proofSearch (Int.sub max_depth 1)) *)
+     (* (fun _ => Control.plus (fun () => ( try (eapply or_elim2); proofSearch (Int.sub max_depth 1)); (maybePrintMessage "Trying or_elim2"); proofSearch (Int.sub max_depth 1)) *)
+     (* (fun _ => Control.plus (fun () => ( try (eapply impl_intro); proofSearch (Int.sub max_depth 1)); (maybePrintMessage "Trying impl_intro"); proofSearch (Int.sub max_depth 1)) *)
+     (* (fun _ => Control.plus (fun () => ( try (eapply bot_elim); proofSearch (Int.sub max_depth 1)); (maybePrintMessage "Trying bot_elim"); proofSearch (Int.sub max_depth 1)) *)
+     (* (fun _ => Control.plus (fun () => ( try (eapply assume_bot); proofSearch (Int.sub max_depth 1)); (maybePrintMessage "Trying assume_bot"); proofSearch (Int.sub max_depth 1)) *)
+     (* (fun _ => Control.plus (fun () => ( try (eapply admit ); proofSearch (Int.sub max_depth 1)); (maybePrintMessage "Trying admit"); proofSearch (Int.sub max_depth 1)) *)
      
-     (fun _ => fail )))))))))
+     (fun _ => fail ))))))
      (fun _ => fail )
 end.
 
@@ -908,13 +910,13 @@ Set Default Proof Mode "Ltac2".
 Ltac2 autoProveWithDepth max_depth :=
 proofSearch max_depth.
 
-(* Ltac2 rec autoProveWithProgressiveDepth d :=
+Ltac2 rec autoProveWithProgressiveDepth d :=
 Message.print (Message.of_string "Trying depth:");
 Message.print (Message.of_int d);
 try (autoProveWithDepth d);
-try (autoProveWithProgressiveDepth (Int.add d 1)). *)
+try (autoProveWithProgressiveDepth (Int.add d 1)).
 
-Ltac2 rec autoProveWithProgressiveDepth d :=
+(* Ltac2 rec autoProveWithProgressiveDepth d :=
 Message.print (Message.of_string "Trying depth: 1");
 try (autoProveWithDepth 1);
 Message.print (Message.of_string "Trying depth: 2");
@@ -923,7 +925,7 @@ Message.print (Message.of_string "Trying depth: 3");
 try (autoProveWithDepth 3);
 Message.print (Message.of_string "Trying depth: 4");
 try (autoProveWithDepth 4)
-.
+. *)
 
 Ltac2 autoProve () :=
 eexists _ _ _;
@@ -934,32 +936,29 @@ solve [ apply CQ | apply aQ | apply eQ | apply ([] : list singleJudgement) | app
 
 (* Set Ltac2 Backtrace. *)
 
-(* Definition exampleC1 : proofTreeOfClaim (C1).
+Definition exampleC1 : proofTreeOfClaim (C1).
 Proof.
 autoProve ().
 Unshelve.
 all: fillConstant ().
-Defined. *)
+Show Proof.
+Defined.
 
 (*|
 .. coq:: unfold
    :class: coq-math
 |*)
 
-(* Eval compute in show exampleC1. *)
+Eval compute in show exampleC1.
 
 (*|
 .. coq::
 |*)
 Set Default Proof Mode "Ltac2".
 
-Definition automatedProof : proofTreeOfClaim (C1 /\' C2 /\' C3).
+Definition automatedProof : proofTreeOfClaim (C1 /\' C2 /\' C3 /\' C4 /\' C5).
 Proof.
-eexists _ _ _.
-eapply and_intro.
-eapply and_intro.
-all: eapply assume.
-all: eapply leaf.
+autoProve ().
 Unshelve.
 all: fillConstant ().
 Show Proof.
